lack of proof star

LTS.thy
@@ -1,4 +1,3 @@
-
 theory LTS
 imports Main "HOL.Option"
 begin
@@ -11,8 +10,9 @@ a labeled transition system is a subset of $\mathcal{Q} \times \Sigma
 q')$ is an element of $\Delta$ iff starting in state $q$ the state
 $q'$ can be reached reading the label $\sigma$. \<close>
 
-  
+
 type_synonym ('q,'a) LTS = "('q * 'a set * 'q) set"
+
 
 subsubsection  \<open>Reachability\<close>
 
@@ -20,104 +20,13 @@ text \<open>Often it is enough to consider just the first and last state of
 a path. This leads to the following definition of reachability. Notice, 
 that @{term "LTS_is_reachable \<Delta>"} is the reflexive, transitive closure of @{term \<Delta>}.\<close>
 
-inductive LTS_is_reachable :: "('q, 'a) LTS \<Rightarrow>  ('q * 'q) set \<Rightarrow> 'q \<Rightarrow> 'a list \<Rightarrow> 'q \<Rightarrow> bool" for \<Delta> and \<Delta>' where
-  LTS_Empty[intro!]: "LTS_is_reachable \<Delta> \<Delta>' q [] q" |
-  LTS_Step1: "LTS_is_reachable \<Delta> \<Delta>' q l q'" if "(q, q'') \<in> \<Delta>'" and "LTS_is_reachable \<Delta> \<Delta>' q'' l q'" |
-  LTS_Step2[intro!]: "LTS_is_reachable \<Delta> \<Delta>' q (a # w) q'" if "a \<in> \<sigma>" and "(q, \<sigma>, q'') \<in> \<Delta>" and "LTS_is_reachable \<Delta> \<Delta>' q'' w q'"
+primrec LTS_is_reachable :: "('q, 'a) LTS \<Rightarrow> 'q \<Rightarrow> 'a list \<Rightarrow> 'q \<Rightarrow> bool" where
+   "LTS_is_reachable \<Delta> q [] q' = (q = q' ∨ (q, {}, q') ∈ Δ)"|
+   "LTS_is_reachable \<Delta> q (a # w) q' =
+      (\<exists>q'' \<sigma>. a \<in> \<sigma> \<and> (q, \<sigma>, q'') \<in> \<Delta> \<and> LTS_is_reachable \<Delta> q'' w q')"
 
 
-thm LTS_is_reachable.cases 
-thm LTS_is_reachable.induct
+lemma LChr_lemma :"LTS_is_reachable {(a,{x},b)} a l b ⟹ a≠ b ⟹ l = [x]"
+  by (smt (verit, del_insts) LTS_is_reachable.simps(1) LTS_is_reachable.simps(2) empty_iff old.prod.inject remdups_adj.cases singleton_iff)
 
-lemma removeExtraConstrans: "LTS_is_reachable \<Delta> (insert (e1, e2) \<Delta>') ini l end \<Longrightarrow> \<forall>q \<sigma>. (q, \<sigma>, e1) \<notin> \<Delta> \<Longrightarrow> \<forall>q. (q, e1) \<notin> \<Delta>' \<Longrightarrow> ini \<noteq> e1 \<Longrightarrow> LTS_is_reachable \<Delta> \<Delta>' ini l end"
-  proof (induction rule: LTS_is_reachable.induct)
-    case (LTS_Empty q)
-    then show ?case by auto
-  next
-    case (LTS_Step1 q q'' l q')
-    then show ?case 
-      by (metis LTS_is_reachable.LTS_Step1 insert_iff prod.inject)
-  next
-    case (LTS_Step2 a \<sigma> q q'' w q')
-    then show ?case by auto
-  qed
-
-lemma removeExtraTrans1: "LTS_is_reachable (\<Delta>1 \<union> \<Delta>2) (\<Delta>1' \<union> \<Delta>2') ini l end \<Longrightarrow> \<Delta>1 = \<Delta>2 \<Longrightarrow> \<Delta>1' = \<Delta>2' \<Longrightarrow> LTS_is_reachable \<Delta>1 \<Delta>1' ini l end "
-  by simp
-
-lemma removeExtraTrans2: "LTS_is_reachable (\<Delta>1 \<union> \<Delta>2) (\<Delta>1' \<union> \<Delta>2') ini l end \<Longrightarrow> \<Delta>1 \<noteq> \<Delta>2 \<Longrightarrow> \<Delta>1' = \<Delta>2' \<Longrightarrow> LTS_is_reachable (\<Delta>1 \<union> \<Delta>2) \<Delta>1' ini l end "
-  by simp
-
-lemma removeExtraTrans3: "LTS_is_reachable (\<Delta>1 \<union> \<Delta>2) (\<Delta>1' \<union> \<Delta>2') ini l end \<Longrightarrow> \<Delta>1 \<noteq> \<Delta>2 \<Longrightarrow> \<Delta>1' \<noteq> \<Delta>2' \<Longrightarrow> LTS_is_reachable (\<Delta>1 \<union> \<Delta>2) \<Delta>1' ini l end "
-  sorry
-
-
-lemma Delta1Empty: "LTS_is_reachable d1 d2 p l q \<Longrightarrow> d1 =  {} \<Longrightarrow> l = []"
-  by (induction rule: LTS_is_reachable.induct) auto 
-
-  
-
-lemma subLTSlemma:"LTS_is_reachable \<Delta> \<Delta>' q x y \<Longrightarrow> LTS_is_reachable ( \<Delta> \<union> l1) (\<Delta>' \<union> l2) q x y"
-  proof (induction rule: LTS_is_reachable.induct)
-    case (LTS_Empty q)
-    then show ?case by auto
-  next
-    case (LTS_Step1 q q'' l q')
-    then show ?case 
-      by (meson LTS_is_reachable.LTS_Step1 UnI1)
-  next
-    case (LTS_Step2 a \<sigma> q q'' w q')
-    then show ?case by auto
-  qed
- 
-lemma subLTSlemma1:"LTS_is_reachable \<Delta> \<Delta>' q x y \<Longrightarrow> LTS_is_reachable (\<Delta> \<union> {(f q a, va, f q' a)|q va q'. (q,va,q') \<in> \<Delta>}) (\<Delta>' \<union> l1) q x y"
-  by (simp add: subLTSlemma)
-
-
-lemma DeltLTSlemma1:"LTS_is_reachable \<Delta> \<Delta>' q l q' \<Longrightarrow> LTS_is_reachable ({(f q a, va, f q' a)| q va q'. (q, va, q') \<in> \<Delta>}) ({(f q a, f q' a)| q q'. (q, q') \<in> \<Delta>'}) (f q a) l (f q' a)"
-proof (induction rule: LTS_is_reachable.induct)
-  case (LTS_Empty q)
-  then show ?case by auto
-next
-  case (LTS_Step1 q q'' l q')
-  then show ?case 
-    using LTS_is_reachable.simps by fastforce
-next
-  case (LTS_Step2 a \<sigma> q q'' w q')
-  then show ?case by auto
-qed
-
-
-lemma try1: "LTS_is_reachable  \<Delta> \<Delta>' q l q' \<Longrightarrow>  LTS_is_reachable  \<Delta> (\<Delta>' \<union> a ) q l q'"
-  by (metis subLTSlemma sup.idem)
-
-lemma DeltLTSlemma2:"\<exists>l. LTS_is_reachable \<Delta> \<Delta>' q l q' \<Longrightarrow> \<exists>l. LTS_is_reachable ({(f q a, va, f q' a)| q va q'. (q, va, q') \<in> \<Delta>}) ({(f q a, f q' a)| q q'. (q, q') \<in> \<Delta>'}) (f q a) l (f q' a)"
-  apply(rule exE) apply auto subgoal for la  proof -
-    assume "LTS_is_reachable \<Delta> \<Delta>' q la q'" 
-    then have "LTS_is_reachable {(f q a, va, f q' a) |q va q'. (q, va, q') \<in> \<Delta>} {(f q a, f q' a) |q q'. (q, q') \<in> \<Delta>'} (f q a) la (f q' a)" apply(rule LTS_is_reachable.induct)
-      subgoal by auto
-      subgoal for q q'' l q'
-        using LTS_is_reachable.simps by fastforce
-      subgoal for aa \<sigma> q q'' w q'
-        by auto
-      done
-    then show ?thesis by auto
-  qed
-  done
- 
-
-lemma joinLTSlemma:"LTS_is_reachable  \<Delta> \<Delta>' q x p \<Longrightarrow>  LTS_is_reachable  \<Delta> \<Delta>' p y q''\<Longrightarrow> LTS_is_reachable  \<Delta> \<Delta>' q (x@y) q''"
-proof (induction rule: LTS_is_reachable.induct)
-case (LTS_Empty q)
-then show ?case by auto
-next
-  case (LTS_Step1 q q'' l q')
-then show ?case  by (meson LTS_is_reachable.LTS_Step1)
-next
-  case (LTS_Step2 a \<sigma> q q'' w q')
-  then show ?case by auto
-qed
-
-lemma joinLTSlemma1:"\<exists>x. LTS_is_reachable  \<Delta> \<Delta>' q x p \<Longrightarrow>  \<exists>y. LTS_is_reachable  \<Delta> \<Delta>' p y q''\<Longrightarrow> \<exists>x y. LTS_is_reachable  \<Delta> \<Delta>' q (x@y) q''"
-  by (meson joinLTSlemma)     
 end
