NFA.thy
@@ -16,25 +16,34 @@ begin
 record ('q,'a) NFA_rec =
   \<Q> :: "'q set"           (* "The set of states" *)
   \<Sigma> :: "'a set"           (* alphabet *)
-  \<Delta> :: "('q,'a) LTS"      (* "The transition relation" *)
-  \<Delta>' :: "('q * 'q) set"      (* "The transition relation" *)
+  \<Delta> :: "(('q,'a) LTS * 'q * 'q) list set"      (* "The transition relation" *)
   \<I> :: "'q set"            (* "The set of initial states *)
   \<F> :: "'q set"           (* "The set of final states *)
 
 text \<open>Using notions for labelled transition systems, 
 it is easy to define the languages accepted by automata.\<close>
 
-definition NFA_accept :: "('q, 'a) NFA_rec \<Rightarrow> 'a list \<Rightarrow> bool" where
-  "NFA_accept \<A> w = (\<exists> q \<in> (\<I> \<A>). \<exists> q' \<in> (\<F> \<A>).
-                  LTS_is_reachable (\<Delta> \<A>) (\<Delta>' \<A>) q w q') "
+primrec single_LTS_reachable_by_path :: "'a list ⇒ (('q,'a) LTS * 'q * 'q) list  ⇒ bool " where
+"single_LTS_reachable_by_path w []= (w = [])"|
+"single_LTS_reachable_by_path w (x# xs) = (∃p q. (w = p @ q ∧ LTS_is_reachable (fst x) (fst (snd x)) p (snd (snd x)) ∧ single_LTS_reachable_by_path q xs))"
 
-definition NFA_accept_Q :: "('q, 'a) NFA_rec \<Rightarrow> 'q  \<Rightarrow> 'a list \<Rightarrow> bool" where
-  "NFA_accept_Q \<A> q w = (\<exists> q' \<in> (\<F> \<A>).
-                  LTS_is_reachable (\<Delta> \<A>) (\<Delta>' \<A>) q w q') "
+lemma concat_lemma:"single_LTS_reachable_by_path qa x ⟹ single_LTS_reachable_by_path q xa ⟹ single_LTS_reachable_by_path (qa @ q) (x @ xa)"
+  apply(induct x arbitrary:qa) apply auto apply(induct xa arbitrary:q) apply auto 
+  by metis 
+
+
+lemma inverse_concat_lemma: "single_LTS_reachable_by_path q (xa @ y) ⟹ ∃p qa. q = qa @ p ∧ single_LTS_reachable_by_path qa xa ∧ single_LTS_reachable_by_path p y"
+  apply(induct xa arbitrary:q) apply auto 
+  by (metis append.assoc)
+
+fun judge ::"bool set \<Rightarrow> bool" where
+"judge bs = (True \<in> bs)"
+
+lemma ""
+
+definition NFA_accept :: "('a, 'b) NFA_rec \<Rightarrow> 'b list \<Rightarrow> bool" where
+  "NFA_accept \<A> w = judge ((single_LTS_reachable_by_path w) `  (Δ 𝒜))"
 
 definition \<L> where "\<L> \<A> = {w. NFA_accept \<A> w}"
 
-
-definition LQ :: "('q, 'a) NFA_rec => 'q \<Rightarrow> 'a list set" where 
- "LQ \<A> q = {w. NFA_accept_Q \<A> q w}"
 end
